hax-lib/proof-libs/fstar/core/Core_models.Iter.Sources.Repeat_with.fst
@@ -16,32 +16,14 @@ let repeat_with
     : t_RepeatWith v_F = { f_repeater = repeater } <: t_RepeatWith v_F
 
 [@@ FStar.Tactics.Typeclasses.tcinstance]
+assume
+val impl': #v_A: Type0 -> #v_F: Type0 -> {| i0: Core_models.Ops.Function.t_FnMut v_F Prims.unit |}
+  -> Core_models.Iter.Traits.Iterator.t_Iterator (t_RepeatWith v_F)
+
+unfold
 let impl
       (#v_A #v_F: Type0)
       (#[FStar.Tactics.Typeclasses.tcresolve ()]
           i0:
           Core_models.Ops.Function.t_FnMut v_F Prims.unit)
-    : Core_models.Iter.Traits.Iterator.t_Iterator (t_RepeatWith v_F) =
-  {
-    f_Item = v_A;
-    f_next_pre = (fun (self: t_RepeatWith v_F) -> true);
-    f_next_post
-    =
-    (fun (self: t_RepeatWith v_F) (out1: (t_RepeatWith v_F & Core_models.Option.t_Option v_A)) ->
-        true);
-    f_next
-    =
-    fun (self: t_RepeatWith v_F) ->
-      let (tmp0: v_F), (out: v_A) =
-        Core_models.Ops.Function.f_call_mut #v_F
-          #Prims.unit
-          #FStar.Tactics.Typeclasses.solve
-          self.f_repeater
-          (() <: Prims.unit)
-      in
-      let self:t_RepeatWith v_F = { self with f_repeater = tmp0 } <: t_RepeatWith v_F in
-      let hax_temp_output:Core_models.Option.t_Option v_A =
-        Core_models.Option.Option_Some out <: Core_models.Option.t_Option v_A
-      in
-      self, hax_temp_output <: (t_RepeatWith v_F & Core_models.Option.t_Option v_A)
-  }
+     = impl' #v_A #v_F #i0
